theories/expr_semantics.v
@@ -1,9 +1,6 @@
 From Equations Require Import Equations.
 From stdpp Require Export gmap.
 
-(* TODO: remove list of expressions *)
-(* TODO: fixing the set of used protectors as a counter *)
-
 From stbor Require Export lang_base notation.
 
 Set Default Proof Using "Type".
@@ -14,7 +11,7 @@ Set Default Proof Using "Type".
 Fixpoint subst (x : string) (es : expr) (e : expr) : expr :=
   match e with
   | Var y => if bool_decide (y = x) then es else Var y
-  | Lit l => Lit l
+  | Val v => Val v
   (* | Rec f xl e =>
     Rec f xl $ if bool_decide (BNamed x ≠ f ∧ BNamed x ∉ xl) then subst x es e else e *)
   | Call e el => Call (subst x es e) (map (subst x es) el)
@@ -23,7 +20,6 @@ Fixpoint subst (x : string) (es : expr) (e : expr) : expr :=
   | Place l tag T => Place l tag T
   (* | App e1 el => App (subst x es e1) (map (subst x es) el) *)
   | BinOp op e1 e2 => BinOp op (subst x es e1) (subst x es e2)
-  | TVal el => TVal (map (subst x es) el)
   | Proj e1 e2 => Proj (subst x es e1) (subst x es e2)
   | Conc e1 e2 => Conc (subst x es e1) (subst x es e2)
   | Copy e => Copy (subst x es e)
@@ -57,13 +53,13 @@ Fixpoint subst_l (xl : list binder) (esl : list expr) (e : expr) : option expr :
   end.
 Arguments subst_l _%binder _ _%E.
 
-Definition subst_v (xl : list binder) (vsl : vec val (length xl))
+Definition subst_v (xl : list binder) (vsl : vec result (length xl))
                    (e : expr) : expr :=
-  Vector.fold_right2 (λ b, subst' b ∘ of_val) e _ (list_to_vec xl) vsl.
+  Vector.fold_right2 (λ b, subst' b ∘ of_result) e _ (list_to_vec xl) vsl.
 Arguments subst_v _%binder _ _%E.
 
-Lemma subst_v_eq (xl : list binder) (vsl : vec val (length xl)) e :
-  Some $ subst_v xl vsl e = subst_l xl (of_val <$> vec_to_list vsl) e.
+Lemma subst_v_eq (xl : list binder) (vsl : vec result (length xl)) e :
+  Some $ subst_v xl vsl e = subst_l xl (of_result <$> vec_to_list vsl) e.
 Proof.
   revert vsl. induction xl=>/= vsl; inv_vec vsl=>//=v vsl. by rewrite -IHxl.
 Qed.
@@ -71,27 +67,26 @@ Qed.
 (** Evaluation contexts *)
 Inductive ectx_item :=
 (* | AppLCtx (el : list expr) *)
-(* | AppRCtx (v : val) (vl : list val) (el : list expr) *)
+(* | AppRCtx (r : result) (rl : list result) (el : list expr) *)
 | CallLCtx (el: list expr)
-| CallRCtx (v : val) (vl : list val) (el : list expr)
+| CallRCtx (r : result) (rl : list result) (el : list expr)
 | EndCallCtx
 | BinOpLCtx (op : bin_op) (e2 : expr)
-| BinOpRCtx (op : bin_op) (v1 : val)
-| TValCtx (vl : list val) (el : list expr)
+| BinOpRCtx (op : bin_op) (r1 : result)
 | ProjLCtx (e : expr)
-| ProjRCtx (v : val)
+| ProjRCtx (r : result)
 | ConcLCtx (e : expr)
-| ConcRCtx (v : val)
+| ConcRCtx (r : result)
 | CopyCtx
 | WriteLCtx (e : expr)
-| WriteRCtx (v : val)
+| WriteRCtx (r : result)
 | FreeCtx
 (* | CasLCtx (e1 e2: expr) *)
-(* | CasMCtx (v0 : val) (e2 : expr) *)
-(* | CasRCtx (v0 : val) (v1 : val) *)
+(* | CasMCtx (r0 : result) (e2 : expr) *)
+(* | CasRCtx (r0 : result) (r1 : result) *)
 (* | AtRdCtx *)
 (* | AtWrLCtx (e : expr) *)
-(* | AtWrRCtx (v : val) *)
+(* | AtWrRCtx (r : result) *)
 | DerefCtx (T: type)
 | RefCtx
 | FieldCtx (path : list nat)
@@ -102,27 +97,26 @@ Inductive ectx_item :=
 Definition fill_item (Ki : ectx_item) (e : expr) : expr :=
   match Ki with
   (* | AppLCtx el => App e el *)
-  (* | AppRCtx v vl el => App (of_val v) ((of_val <$> vl) ++ e :: el) *)
+  (* | AppRCtx r rl el => App (of_result r) ((of_result <$> rl) ++ e :: el) *)
   | CallLCtx el => Call e el
-  | CallRCtx v vl el => Call (of_val v) ((of_val <$> vl) ++ e :: el)
+  | CallRCtx r rl el => Call (of_result r) ((of_result <$> rl) ++ e :: el)
   | EndCallCtx => EndCall e
   | BinOpLCtx op e2 => BinOp op e e2
-  | BinOpRCtx op v1 => BinOp op (of_val v1) e
-  | TValCtx vl el => TVal ((of_val <$> vl) ++ e :: el)
+  | BinOpRCtx op r1 => BinOp op (of_result r1) e
   | ProjLCtx e2 => Proj e e2
-  | ProjRCtx v1 => Proj (of_val v1) e
+  | ProjRCtx r1 => Proj (of_result r1) e
   | ConcLCtx e2 => Conc e e2
-  | ConcRCtx v1 => Conc (of_val v1) e
+  | ConcRCtx r1 => Conc (of_result r1) e
   | CopyCtx => Copy e
   | WriteLCtx e2 => Write e e2
-  | WriteRCtx v1 => Write (of_val v1) e
+  | WriteRCtx r1 => Write (of_result r1) e
   | FreeCtx => Free e
   (* | CasLCtx e1 e2 => CAS e e1 e2 *)
-  (* | CasMCtx v0 e2 => CAS (of_val v0) e e2 *)
-  (* | CasRCtx v0 v1 => CAS (of_val v0) (of_val v1) e *)
+  (* | CasMCtx v0 e2 => CAS (of_result v0) e e2 *)
+  (* | CasRCtx v0 v1 => CAS (of_result v0) (of_result v1) e *)
   (* | AtRdCtx => AtomRead e *)
   (* | AtWrLCtx e2 => AtomWrite e e2 *)
-  (* | AtWrRCtx v1 => AtomWrite (of_val v1) e *)
+  (* | AtWrRCtx v1 => AtomWrite (of_result v1) e *)
   | DerefCtx T => Deref e T
   | RefCtx => Ref e
   | FieldCtx path => Field e path
@@ -137,18 +131,18 @@ Definition fill_item (Ki : ectx_item) (e : expr) : expr :=
 Definition Z_of_bool (b : bool) : Z :=
   if b then 1 else 0.
 
-Definition lit_of_bool (b : bool) : lit :=
-  LitInt $ Z_of_bool b.
+Definition sc_of_bool (b : bool) : scalar :=
+  ScInt $ Z_of_bool b.
 
-Coercion lit_of_bool : bool >-> lit.
-Coercion LitInt : Z >-> lit.
+Coercion sc_of_bool : bool >-> scalar.
+Coercion ScInt : Z >-> scalar.
 
 Implicit Type (h: mem).
 
 Fixpoint init_mem (l:loc) (n:nat) h : mem :=
   match n with
   | O => h
-  | S n => <[l := LitPoison]>(init_mem (l +ₗ 1) n h)
+  | S n => <[l := ☠%S]>(init_mem (l +ₗ 1) n h)
   end.
 
 Fixpoint free_mem (l:loc) (n:nat) h : mem :=
@@ -157,10 +151,10 @@ Fixpoint free_mem (l:loc) (n:nat) h : mem :=
   | S n => delete l (free_mem (l +ₗ 1) n h)
   end.
 
-Inductive lit_eq h : lit → lit → Prop :=
+Inductive scalar_eq h : scalar → scalar → Prop :=
 (* No refl case for poison *)
-| IntRefl z : lit_eq h (LitInt z) (LitInt z)
-| LocRefl l tag1 tag2 : lit_eq h (LitLoc l tag1) (LitLoc l tag2)
+| IntRefl z : scalar_eq h (ScInt z) (ScInt z)
+| LocRefl l tag1 tag2 : scalar_eq h (ScPtr l tag1) (ScPtr l tag2)
 (* Comparing unallocated pointers can non-deterministically say they are equal
    even if they are not.  Given that our `free` actually makes addresses
    re-usable, this may not be strictly necessary, but it is the most
@@ -170,36 +164,36 @@ Inductive lit_eq h : lit → lit → Prop :=
    more background. *)
 | LocUnallocL l1 l2 tag1 tag2 :
     h !! l1 = None →
-    lit_eq h (LitLoc l1 tag1) (LitLoc l2 tag2)
+    scalar_eq h (ScPtr l1 tag1) (ScPtr l2 tag2)
 | LocUnallocR l1 l2 tag1 tag2 :
     h !! l2 = None →
-    lit_eq h (LitLoc l1 tag1) (LitLoc l2 tag2).
+    scalar_eq h (ScPtr l1 tag1) (ScPtr l2 tag2).
 
-Inductive lit_neq : lit → lit → Prop :=
+Inductive scalar_neq : scalar → scalar → Prop :=
 | IntNeq z1 z2 :
-    z1 ≠ z2 → lit_neq (LitInt z1) (LitInt z2)
+    z1 ≠ z2 → scalar_neq (ScInt z1) (ScInt z2)
 | LocNeq l1 l2 tag1 tag2 :
-    l1 ≠ l2 → lit_neq (LitLoc l1 tag1) (LitLoc l2 tag2)
+    l1 ≠ l2 → scalar_neq (ScPtr l1 tag1) (ScPtr l2 tag2)
 | LocNeqNullR l tag :
-    lit_neq (LitLoc l tag) (LitInt 0)
+    scalar_neq (ScPtr l tag) (ScInt 0)
 | LocNeqNullL l tag :
-    lit_neq (LitInt 0) (LitLoc l tag).
+    scalar_neq (ScInt 0) (ScPtr l tag).
 
-Inductive bin_op_eval h : bin_op → lit → lit → lit → Prop :=
+Inductive bin_op_eval h : bin_op → scalar → scalar → scalar → Prop :=
 | BinOpPlus z1 z2 :
-    bin_op_eval h AddOp (LitInt z1) (LitInt z2) (LitInt (z1 + z2))
+    bin_op_eval h AddOp (ScInt z1) (ScInt z2) (ScInt (z1 + z2))
 | BinOpMinus z1 z2 :
-    bin_op_eval h SubOp (LitInt z1) (LitInt z2) (LitInt (z1 - z2))
+    bin_op_eval h SubOp (ScInt z1) (ScInt z2) (ScInt (z1 - z2))
 | BinOpLe z1 z2 :
-    bin_op_eval h LeOp (LitInt z1) (LitInt z2) (lit_of_bool $ bool_decide (z1 ≤ z2))
+    bin_op_eval h LeOp (ScInt z1) (ScInt z2) (sc_of_bool $ bool_decide (z1 ≤ z2))
 | BinOpLt z1 z2 :
-    bin_op_eval h LtOp (LitInt z1) (LitInt z2) (lit_of_bool $ bool_decide (z1 < z2))
+    bin_op_eval h LtOp (ScInt z1) (ScInt z2) (sc_of_bool $ bool_decide (z1 < z2))
 | BinOpEqTrue l1 l2 :
-    lit_eq h l1 l2 → bin_op_eval h EqOp l1 l2 (lit_of_bool true)
+    scalar_eq h l1 l2 → bin_op_eval h EqOp l1 l2 (sc_of_bool true)
 | BinOpEqFalse l1 l2 :
-    lit_neq l1 l2 → bin_op_eval h EqOp l1 l2 (lit_of_bool false)
+    scalar_neq l1 l2 → bin_op_eval h EqOp l1 l2 (sc_of_bool false)
 | BinOpOffset l z tag :
-    bin_op_eval h OffsetOp (LitLoc l tag) (LitInt z) (LitLoc (l +ₗ z) tag).
+    bin_op_eval h OffsetOp (ScPtr l tag) (ScInt z) (ScPtr (l +ₗ z) tag).
 
 (* Compute subtype of `T` and offset to it from `path` *)
 Fixpoint field_access (T: type) (path : list nat) :
@@ -208,8 +202,8 @@ Fixpoint field_access (T: type) (path : list nat) :
   | [] => Some (O, T)
   | i :: path =>
     match T with
-    | Scalar sz =>
-        if bool_decide (i ≤ sz) then Some (i, Scalar (sz - i)) else None
+    | FixedSize sz =>
+        if bool_decide (i ≤ sz) then Some (i, FixedSize (sz - i)) else None
     | Reference _ _ => match i with O => Some (O, T) | _ => None end
     | Unsafe T => field_access T path
     | Union Ts => T ← Ts !! i ; field_access T path
@@ -222,15 +216,15 @@ Fixpoint field_access (T: type) (path : list nat) :
     end
   end.
 
-Fixpoint write_mem l (vl: list lit) h: mem :=
-  match vl with
+Fixpoint write_mem l (v: value) h: mem :=
+  match v with
   | [] => h
-  | v :: vl => write_mem (l +ₗ 1) vl (<[l := v]> h)
+  | s :: v => write_mem (l +ₗ 1) v (<[l := s]> h)
   end.
 
-Equations read_mem (l: loc) (n: nat) h: option (list lit) :=
+Equations read_mem (l: loc) (n: nat) h: option value :=
   read_mem l n h := go l n (Some [])
-  where go : loc → nat → option (list lit) → option (list lit) :=
+  where go : loc → nat → option value → option value :=
         go l O      oacc := oacc;
         go l (S n)  oacc :=
           acc ← oacc ;
@@ -252,42 +246,39 @@ Proof.
 Qed.
 
 Inductive pure_expr_step (FNs: fn_env) (h: mem) : expr → event → expr → Prop :=
-| BinOpPS op l1 l2 l' :
+| BinOpPS op (l1 l2 l': scalar) :
     bin_op_eval h op l1 l2 l' →
-    pure_expr_step FNs h (BinOp op (#[ #l1]) (#[ #l2])) SilentEvt (#[ #l'])
-(* TODO: add more operations for tempvalue lists *)
-| ProjBS el (i: Z) vl v
-    (DEFINED: 0 ≤ i ∧ vl !! (Z.to_nat i) = Some v)
-    (VALUES: to_val (TVal el) = Some (TValV vl)) :
-    pure_expr_step FNs h (Proj (TVal el) #i) SilentEvt #v
-| ConcBS el1 el2 vl1 vl2
-    (VALUES1: to_val (TVal el1) = Some (TValV vl1))
-    (VALUES2: to_val (TVal el2) = Some (TValV vl2)) :
-    pure_expr_step FNs h (Conc (TVal el1) (TVal el2))
-                         SilentEvt (of_val (TValV (vl1 ++ vl2)))
+    pure_expr_step FNs h (BinOp op (#[l1]) (#[l2])) SilentEvt (#[l'])
+(* TODO: add more operations for values *)
+| ProjBS (i: Z) (v : value) (s : scalar)
+    (DEFINED: 0 ≤ i ∧ v !! (Z.to_nat i) = Some s) :
+    pure_expr_step FNs h (Proj (Val v) #[i]) SilentEvt #[s]
+| ConcBS v1 v2 :
+    pure_expr_step FNs h (Conc (Val v1) (Val v2))
+                         SilentEvt (Val (v1 ++ v2))
 | RefBS l lbor T :
     is_Some (h !! l) →
-    pure_expr_step FNs h (Ref (Place l lbor T)) SilentEvt #(LitLoc l lbor)
+    pure_expr_step FNs h (Ref (Place l lbor T)) SilentEvt #[ScPtr l lbor]
 | DerefBS l lbor T
     (DEFINED: ∀ (i: nat), (i < tsize T)%nat → l +ₗ i ∈ dom (gset loc) h) :
-    pure_expr_step FNs h ( *{T} #(LitLoc l lbor)) SilentEvt (Place l lbor T)
+    pure_expr_step FNs h ( *{T} #[ScPtr l lbor]) SilentEvt (Place l lbor T)
 | FieldBS l lbor T path off T'
     (FIELD: field_access T path = Some (off, T')) :
     pure_expr_step FNs h (Field (Place l lbor T) path)
                          SilentEvt (Place (l +ₗ off) lbor T')
 | LetBS x e1 e2 e' :
-    is_Some (to_val e1) →
+    is_Some (to_result e1) →
     subst x e2 e1 = e' →
     pure_expr_step FNs h (let: x := e1 in e2) SilentEvt e'
 | CaseBS i el e :
     0 ≤ i →
     el !! (Z.to_nat i) = Some e →
-    pure_expr_step FNs h (case: #i of el) SilentEvt e
+    pure_expr_step FNs h (case: #[i] of el) SilentEvt e
 | CallBS name el xl e HC e':
     FNs !! name = Some (@FunV xl e HC) →
-    Forall (λ ei, is_Some (to_val ei)) el →
+    Forall (λ ei, is_Some (to_value ei)) el →
     subst_l xl el e = Some e' →
-    pure_expr_step FNs h (Call #(LitFnPtr name) el)
+    pure_expr_step FNs h (Call #[ScFnPtr name] el)
                          (NewCallEvt name) (InitCall e').
 
 
@@ -298,23 +289,23 @@ Inductive mem_expr_step (h: mem) : expr → event → mem → expr → Prop :=
               (InitCallEvt c)
               h (EndCall e)
 | EndCallBS (call: call_id) e v:
-    to_val e = Some v →
-    mem_expr_step h (EndCall e) (EndCallEvt call) h v
-| CopyBS l lbor T (vl: list lit)
-    (READ: read_mem l (tsize T) h = Some vl)
-    (* (LEN: length vl = tsize T) *)
-    (* (VALUES: ∀ (i: nat), (i < length vl)%nat → h !! (l +ₗ i) = vl !! i) *) :
+    to_result e = Some (ValR v) →
+    mem_expr_step h (EndCall e) (EndCallEvt call v) h #v
+| CopyBS l lbor T (v: value)
+    (READ: read_mem l (tsize T) h = Some v)
+    (* (LEN: length v = tsize T) : true by read_mem_values *)
+    (* (VALUES: ∀ (i: nat), (i < length v)%nat → h !! (l +ₗ i) = v !! i)
+        : true by read_mem_values *) :
     mem_expr_step
               h (Copy (Place l lbor T))
-              (CopyEvt l lbor T vl)
-              h (of_val (TValV vl))
-| WriteBS l lbor T el vl (LENe: length vl = tsize T)
-    (DEFINED: ∀ (i: nat), (i < length vl)%nat → l +ₗ i ∈ dom (gset loc) h)
-    (VALUES: to_val (TVal el) = Some (TValV vl)) :
+              (CopyEvt l lbor T v)
+              h (Val v)
+| WriteBS l lbor T v (LEN: length v = tsize T)
+    (DEFINED: ∀ (i: nat), (i < length v)%nat → l +ₗ i ∈ dom (gset loc) h) :
     mem_expr_step
-              h (Place l lbor T <- TVal el)
-              (WriteEvt l lbor T vl)
-              (write_mem l vl h) #☠
+              h (Place l lbor T <- Val v)
+              (WriteEvt l lbor T v)
+              (write_mem l v h) #[☠]
 | AllocBS lbor T :
     let l := (fresh_block h, 0) in
     mem_expr_step
@@ -326,12 +317,12 @@ Inductive mem_expr_step (h: mem) : expr → event → mem → expr → Prop :=
     mem_expr_step
               h (Free (Place l lbor T))
               (DeallocEvt l lbor T)
-              (free_mem l (tsize T) h) #☠
+              (free_mem l (tsize T) h) #[☠]
 | RetagBS x xbor T kind :
     mem_expr_step
               h (Retag (Place x xbor T) kind)
               (RetagEvt x T kind)
-              h (Lit LitPoison)
+              h #[☠]
 (* | ForkBS e h:
     expr_step (Fork e) h SilentEvt (Lit LitPoison) h [e] *)
 (* observable behavior *)
