theories/properties.v
@@ -6,34 +6,34 @@ Set Default Proof Using "Type".
 Class Wellformed A := Wf : A → Prop.
 Existing Class Wf.
 
-Definition wf_mem_tag (h: mem) (clk: ptr_id) :=
-  ∀ l l' bor, h !! l = Some (LitLoc l' bor) → bor <b clk.
+Definition wf_mem_tag (h: mem) (nxtp: ptr_id) :=
+  ∀ l l' bor, h !! l = Some (ScPtr l' bor) → bor <b nxtp.
 
-Definition stack_item_included (stk: stack) (β: protectors) (clk: ptr_id) :=
+Definition stack_item_included (stk: stack) (nxtp: ptr_id) (nxtc: call_id) :=
   ∀ si, si ∈ stk → match si.(tg) with
-                    | Tagged t => (t < clk)%nat
+                    | Tagged t => (t < nxtp)%nat
                     | _ => True
                    end ∧
                    match si.(protector) with
-                    | Some c => c ∈ β
+                    | Some c => (c < nxtc)%nat
                     | _ => True
                    end.
-Definition wf_stack_item (α: stacks) (β: protectors) (clk: ptr_id) :=
-  ∀ l stk, α !! l = Some stk → stack_item_included stk β clk.
+Definition wf_stack_item (α: stacks) (nxtp: ptr_id) (nxtc: call_id) :=
+  ∀ l stk, α !! l = Some stk → stack_item_included stk nxtp nxtc.
 Definition wf_non_empty (α: stacks) :=
   ∀ l stk, α !! l = Some stk → stk ≠ [].
 Definition wf_no_dup (α: stacks) :=
   ∀ l stk, α !! l = Some stk → NoDup stk.
-Definition wf_cid_pro (cids: call_id_stack) (β: protectors) :=
-  ∀ c : call_id, c ∈ cids → c ∈ β.
+Definition wf_cid_incl (cids: call_id_stack) (nxtc: call_id) :=
+  ∀ c : call_id, c ∈ cids → (c < nxtc)%nat.
 
 Record state_wf' (s: state) := {
   state_wf_dom : dom (gset loc) s.(shp) ≡ dom (gset loc) s.(sst);
-  state_wf_mem_tag : wf_mem_tag s.(shp) s.(scn);
-  state_wf_stack_item : wf_stack_item s.(sst) s.(spr) s.(scn);
+  state_wf_mem_tag : wf_mem_tag s.(shp) s.(snp);
+  state_wf_stack_item : wf_stack_item s.(sst) s.(snp) s.(snc);
   state_wf_non_empty : wf_non_empty s.(sst);
   state_wf_cid_no_dup : NoDup s.(scs) ;
-  state_wf_cid_agree: wf_cid_pro s.(scs) s.(spr);
+  state_wf_cid_agree: wf_cid_incl s.(scs) s.(snc);
   (* state_wf_cid_non_empty : s.(scs) ≠ []; *)
   (* state_wf_no_dup : wf_no_dup σ.(cst).(sst); *)
 }.
@@ -42,12 +42,12 @@ Instance state_wf : Wellformed state :=  state_wf'.
 Instance config_wf : Wellformed config := λ cfg, Wf cfg.(cst).
 Notation terminal e := (is_Some (to_val e)).
 
-Lemma expr_terminal_False (e: expr) : ¬ terminal e ↔ to_val e = None.
+Lemma expr_terminal_False (e: expr) : ¬ terminal e ↔ to_result e = None.
 Proof.
   split.
   - destruct (to_val e) eqn:Eqv; [|done].
     intros TERM. exfalso. apply TERM. by eexists.
-  - intros Eq1 [? Eq2]. by rewrite Eq1 in Eq2.
+  - intros Eq1 [? Eq2]. by rewrite /to_val /= Eq1 in Eq2.
 Qed.
 
 (** Thread steps *)
